\documentclass[12pt]{article}
\usepackage{lipsum}
\usepackage{amsmath}
\usepackage{amsthm}

\newtheoremstyle{mystyle}%                % Name
  {}%                                     % Space above
  {}%                                     % Space below
  {\itshape}%                             % Body font
  {}%                                     % Indent amount
  {\bfseries}%                            % Theorem head font
  {.}%                                    % Punctuation after theorem head
  { }%                                    % Space after theorem head, ' ', or \newline
  {}%                                     % Theorem head spec (can be left empty, meaning `normal')

\theoremstyle{mystyle}
\newtheorem{thm}[equation]{Theorem}
\newtheorem{cor}[equation]{Corollary}
\newtheorem{lemma}[equation]{Lemma}
\newtheorem{prop}[equation]{Proposition}
\newtheorem{conj}[equation]{Conjecture}
\newtheorem{definition}[equation]{Definition}
\newtheorem{remark}[equation]{Remark}
\newtheorem{example}[equation]{Example}

\usepackage{graphicx}
\usepackage[margin=1in,footskip=0.25in]{geometry}
\usepackage{hyperref}
\usepackage[utf8]{inputenc}
\title{OP202 HW}
\author{Yanyu ZHOU}
\date{\today}

\begin{document}
\maketitle
\section{Q1}
\begin{example}
   $ -\log(x)$ is self-confordant on its own domain but not strongly convex.
\end{example}

\begin{proof}
    Let $f(x) = -\log(x), x >0$, then $f^\prime (x) = -\frac{1}{x}$, $f^{\prime \prime} (x) = x^{-2}$, $f^{\prime \prime \prime} (x) = -2x^{-3}$.
    Since $2x^{-3} \leq 2x^{-3}$, $|-2x^{-3}| \leq f^{\prime \prime} (x)^{\frac{3}{2}}$.

    Also, if there exists a $m > 0 $ such that $f$ is m-strongly convex, we have $f^{\prime \prime} (x) \geq m\text{In}$. It's impossible since $x>0$.
\end{proof}
\section{Q2}
\begin{thm}
All positive semi-definite matrices form a convex set.
\end{thm}

\begin{proof}
    Let A, B be two positive semi-definite matrices, $\lambda \in [0,1]$. Then we have
    $$x^T [\lambda A + (1-\lambda)B]x = x^T(\lambda Ax + (1-\lambda)Bx) = \lambda x^T Ax+ (1-\lambda)x^TBx \geq 0.$$
\end{proof}

\end{document}